Finally finish 3.10.2 and add instance BEq (Term sig X)
Some recursion problems again that could be circumvented with mutual...
Also the forward direction for 3.10.2 feels somewhat convoluted, maybe the proof for the lemma could be made more elegant at a later time?

InferenceInLean/Syntax.lean
@@ -43,8 +43,26 @@ lemma Term.induction {sig : Signature} {X : Variables} {P : (Term sig X) → Pro
       intro term' harg'
       exact ih term' harg'
 
+mutual
+  def eqTerm {sig : Signature} {X : Variables} [instX : BEq X] [instF : BEq sig.funs] :
+      Term sig X → Term sig X → Bool
+    | Term.var x, Term.var y => x == y
+    | Term.func f fargs, Term.func g gargs => f == g && eqArgs fargs gargs
+    | _, _ => false
+  def eqArgs {sig : Signature} {X : Variables} [instX : BEq X] [instF : BEq sig.funs] :
+      List (Term sig X) → List (Term sig X) → Bool
+    | [], [] => true
+    | [], _ => false
+    | _, [] => false
+    | x :: xs, y :: ys => eqTerm x y && eqArgs xs ys
+end
+
+instance {sig : Signature} {X : Variables} [instX : BEq X] [instF : BEq sig.funs] :
+    BEq (Term sig X) :=
+  ⟨eqTerm⟩
+
 @[simp]
-def Term.freeVars {sig : Signature} {X : Variables} : @Term sig X -> Set X
+def Term.freeVars {sig : Signature} {X : Variables} : Term sig X -> Set X
   | .var x => {x}
   | .func _ [] => ∅
   | .func f (a :: args) => Term.freeVars a ∪ Term.freeVars (Term.func f args)
@@ -54,13 +72,13 @@ inductive Atom (sig : Signature) (X : Variables) where
   | eq (lhs rhs : Term sig X)
 
 @[simp]
-def Atom.freeVars {sig : Signature} {X : Variables} : @Atom sig X -> Set X
+def Atom.freeVars {sig : Signature} {X : Variables} : Atom sig X -> Set X
   | .pred _ args => args.foldl (fun acc t => acc ∪ Term.freeVars t) ∅
   | .eq lhs rhs => Term.freeVars lhs ∪ Term.freeVars rhs
 
 inductive Literal (sig : Signature) (X : Variables) where
-  | pos (a : @Atom sig X)
-  | neg (a : @Atom sig X)
+  | pos (a : Atom sig X)
+  | neg (a : Atom sig X)
 
 @[simp]
 def Literal.comp {sig : Signature} {X : Variables} : Literal sig X -> Literal sig X
@@ -82,14 +100,14 @@ instance {sig : Signature} {X : Variables} : HAppend (Clause sig X) (Clause sig 
 inductive Formula (sig: Signature) (X: Variables) where
   | falsum
   | verum
-  | atom (a : @Atom sig X)
-  | neg (f : @Formula sig X)
-  | and (f g : @Formula sig X)
-  | or (f g : @Formula sig X)
-  | imp (f g : @Formula sig X)
-  | iff (f g : @Formula sig X)
-  | all (x : X) (f : @Formula sig X)
-  | ex (x : X) (f : @Formula sig X)
+  | atom (a : Atom sig X)
+  | neg (f : Formula sig X)
+  | and (f g : Formula sig X)
+  | or (f g : Formula sig X)
+  | imp (f g : Formula sig X)
+  | iff (f g : Formula sig X)
+  | all (x : X) (f : Formula sig X)
+  | ex (x : X) (f : Formula sig X)
 
 /--
  Creates formula ∀ x_1 ... x_n, F.
@@ -102,7 +120,7 @@ def Formula.bigForall {sig : Signature} {X : Variables} [DecidableEq X]
   | x :: xs => .all x (F.bigForall xs)
 
 @[simp]
-def Clause.toFormula {sig : Signature} {X : Variables} : @Clause sig X -> @Formula sig X
+def Clause.toFormula {sig : Signature} {X : Variables} : Clause sig X -> Formula sig X
   | [] => Formula.falsum
   | .pos l :: ls => Formula.or (Formula.atom l) (Clause.toFormula ls)
   | .neg l :: ls => Formula.or (Formula.neg (Formula.atom l)) (Clause.toFormula ls)
@@ -152,11 +170,11 @@ infix:90 " ∘ " => Substitution.compose
 
 @[simp]
 def Substitution.domain {sig : Signature} {X : Variables} (σ : Substitution sig X) : Set X :=
-  {x : X | σ x ≠ Term.var x}
+  {x | σ x ≠ Term.var x}
 
 @[simp]
 def Substitution.codomain {sig : Signature} {X : Variables} (σ : Substitution sig X) : Set X :=
-  {x : X | ∃ y : X, y ∈ σ.domain ∧ x ∈ (σ y).freeVars}
+  {x | ∃ y ∈ σ.domain, x ∈ (σ y).freeVars}
 
 @[simp]
 def MoreGeneral {sig : Signature} {X : Variables} [BEq X] (σ τ : Substitution sig X) : Prop :=
@@ -212,31 +230,58 @@ lemma Substitution.id_of_free_not_in_domain {sig : Signature} {X : Variables} [B
   intro hfreenoindom
   simp_all only [Substitution.domain, ne_eq, Set.mem_setOf_eq, not_not]
   induction' t using Term.induction with x args ih f
-  · simp_all
+  · simp_all only [Term.freeVars, Set.mem_singleton_iff, Term.substitute]
   · induction args <;> simp_all
 
 @[simp]
-theorem idempotent_iff_empty_interesec {sig : Signature} {X : Variables} [BEq X]
+lemma Substitution.ne_subst_of_mem_dom_free {sig : Signature} {X : Variables} [BEq X] [BEq sig.funs]
+    (σ : Substitution sig X) (t : Term sig X) :
+    (∃ x ∈ σ.domain, x ∈ t.freeVars) → t ≠ t.substitute σ := by
+  intro ⟨x,⟨hxindom, hxinfree⟩⟩
+  simp_all
+  by_contra teqtsub
+  induction' t using Term.induction with x' args ih f
+  · rw [Term.substitute.eq_def] at teqtsub
+    simp_all
+    rw [symm teqtsub] at hxinfree
+    simp only [Term.freeVars] at hxinfree
+    subst hxinfree
+    simp_all only [not_true_eq_false]
+  · induction args with
+    | nil =>
+      simp [Term.freeVars] at hxinfree
+    | cons head tail ihargs =>
+      simp only [List.mem_cons, forall_eq_or_imp] at ih
+      obtain ⟨hxinheadimp, hforallintail⟩ := ih
+      have hxintailimp := ihargs hforallintail
+      simp only [Term.substitute, List.attach_cons, List.map_cons, List.map_map,
+        Function.comp_apply, List.map_subtype, List.unattach_attach, Term.func.injEq,
+        List.cons.injEq, true_and] at teqtsub
+      obtain ⟨hheqhsub, hteqsubt⟩ := teqtsub
+      by_cases hxinhead : x ∈ head.freeVars
+      · exact hxinheadimp hxinhead hheqhsub
+      · simp [List.mem_cons, List.cons_inj_right] at hxinfree
+        have hxintail : x ∈ (Term.func f tail).freeVars := or_iff_not_imp_left.mp hxinfree hxinhead
+        have htaileqsubtail := hxintailimp hxintail
+        simp only [Term.substitute, List.map_subtype, List.unattach_attach, Term.func.injEq,
+          true_and] at htaileqsubtail
+        exact htaileqsubtail hteqsubt
+
+@[simp]
+theorem idempotent_iff_inter_empty {sig : Signature} {X : Variables} [BEq X] [BEq sig.funs]
     (σ : Substitution sig X) : Idempotent σ ↔ σ.domain ∩ σ.codomain = ∅ := by
   apply Iff.intro
   -- Forward direction: If σ is idempotent, then its domain and codomain are disjoint.
   · intro hidem
-    simp [*] at hidem
     ext x
-    by_contra hinter
-    simp [*] at hinter
-    obtain ⟨hxindom : x ∈ σ.domain , hxincodom⟩ := hinter
-    obtain ⟨y, ⟨hyindom, hyinfree⟩⟩ := hxincodom
-    have h := congr_fun hidem y
-    /-
-    Do this by counter example:
-    σ={x ↦ y, z ↦ x} => σ.dom = {x, z}, σ.codom = {y, x} => x ∈ σ.codom
-    x maps to something that is not x
-    something maps to x
-    so applying once
-    use that σ z != (σ ∘ σ) z
-    -/
-    sorry
+    apply Iff.intro
+    · simp only [Set.mem_empty_iff_false]
+      intro ⟨hxindom, ⟨y, ⟨hyindom, hxinfree⟩⟩⟩
+      have hidemy := congr_fun hidem y
+      let t := σ y -- construct counterexample
+      have hexists : ∃ x ∈ σ.domain, x ∈ t.freeVars := by aesop
+      exact Substitution.ne_subst_of_mem_dom_free σ t hexists <| symm hidemy
+    · exact fun a ↦ False.elim a
   -- Reverse direction: If the domain and codomain are disjoint, then σ is idempotent.
   · intro h_inter_empty
     have h_disjoint_doms : Disjoint σ.domain σ.codomain := by
@@ -258,3 +303,9 @@ theorem idempotent_iff_empty_interesec {sig : Signature} {X : Variables} [BEq X]
       rw [Substitution.compose]
       refine Substitution.id_of_free_not_in_domain σ (σ x) ?_
       aesop
+
+/-
+Maybe continue with?
+3.3 LEMMA If a is an idempotent substitution and z is an arbitrary substitution, then a is
+more general than z iff za = z.
+-/
